Add intersection on ExtDHashMap

src/Std/Data/ExtDHashMap/Basic.lean
@@ -365,6 +365,20 @@ def union [EquivBEq α] [LawfulHashable α] (m₁ m₂ : ExtDHashMap α β) : Ex
 
 instance [EquivBEq α] [LawfulHashable α] : Union (ExtDHashMap α β) := ⟨union⟩
 
+theorem inter_congr [EquivBEq α] [LawfulHashable α] (a b c d : DHashMap α β) (h₁ : a ~m c) (h₂ : b ~m d) : a ∩ b ~m c ∩ d :=
+  DHashMap.Equiv.trans (DHashMap.inter_equiv_congr_left h₁) (DHashMap.inter_equiv_congr_right h₂)
+
+@[inline, inherit_doc DHashMap.inter]
+def inter [EquivBEq α] [LawfulHashable α] (m₁ m₂ : ExtDHashMap α β) : ExtDHashMap α β := lift₂ (fun x y : DHashMap α β => mk (x.inter y))
+  (fun a b c d equiv₁ equiv₂ => by
+    simp only [DHashMap.inter_eq, mk'.injEq]
+    apply Quotient.sound
+    apply inter_congr
+    · exact equiv₁
+    · exact equiv₂) m₁ m₂
+
+instance [EquivBEq α] [LawfulHashable α] : Inter (ExtDHashMap α β) := ⟨inter⟩
+
 @[inline, inherit_doc DHashMap.Const.unitOfArray]
 def Const.unitOfArray [BEq α] [Hashable α] (l : Array α) :
     ExtDHashMap α (fun _ => Unit) :=
